qcp/ast/VC/alpha_equiv_proof_manual.v
@@ -23,72 +23,206 @@ Local Open Scope sac.
 
 Lemma proof_of_alpha_equiv_entail_wit_1 : alpha_equiv_entail_wit_1.
 Proof.
-    pre_process.
-    unfold termtypeID in *.
-    destruct term1; lia.
+  pre_process.
+  unfold termtypeID in *.
+  destruct term1; lia.
 Qed.
 
 Lemma proof_of_alpha_equiv_return_wit_1_1 : alpha_equiv_return_wit_1_1.
 Proof.
-    pre_process.
-    unfold list_Z_cmp in H0.
-    destruct (list_Z_eqb str1 str2) eqn:Heq; [ contradiction | ].
-    unfold store_term, term_eqn, term_eqb.
-    rewrite H3, H4.
-    Exists y z.
-    entailer!.
-    rewrite Heq.
-    reflexivity.
+  pre_process.
+  unfold list_Z_cmp in H0.
+  destruct (list_Z_eqb str1 str2) eqn:Heq; [ contradiction | ].
+  unfold store_term, term_eqn, term_eqb.
+  rewrite H3, H4.
+  Exists y z.
+  entailer!.
+  rewrite Heq.
+  reflexivity.
 Qed.
 
 Lemma proof_of_alpha_equiv_return_wit_1_2 : alpha_equiv_return_wit_1_2.
 Proof.
-    pre_process.
-    rewrite H in H0.
-    unfold list_Z_cmp in H0.
-    destruct (list_Z_eqb str1 str2) eqn:Heq; [ | discriminate ].
-    unfold store_term, term_eqn, term_eqb.
-    rewrite H3, H4.
-    Exists y z.
-    entailer!.
-    rewrite Heq.
-    reflexivity.
+  pre_process.
+  rewrite H in H0.
+  unfold list_Z_cmp in H0.
+  destruct (list_Z_eqb str1 str2) eqn:Heq; [ | discriminate ].
+  unfold store_term, term_eqn, term_eqb.
+  rewrite H3, H4.
+  Exists y z.
+  entailer!.
+  rewrite Heq.
+  reflexivity.
 Qed.
 
 Lemma proof_of_alpha_equiv_return_wit_2 : alpha_equiv_return_wit_2.
 Proof.
-    pre_process.
-    unfold store_term, term_eqn, term_eqb.
-    rewrite H2, H3.
-    entailer!.    
-    Admitted. 
+  pre_process.
+  unfold store_term, term_eqn, term_eqb.
+  rewrite H2, H3.
+  entailer!.
+  destruct (ctID typ1 =? ctID typ2)%Z eqn:E.
+  + apply Z.eqb_eq in E.
+    contradiction.
+  + rewrite Bool.andb_false_l.
+    reflexivity.
+Qed.
 
 Lemma proof_of_alpha_equiv_return_wit_3_1 : alpha_equiv_return_wit_3_1.
-Proof. Admitted. 
+Proof. 
+  pre_process.
+  unfold store_term.
+  rewrite H4, H5.
+  entailer!.
+  unfold term_eqn, term_eqb.
+  rewrite H1 at 1.
+  rewrite Z.eqb_refl.
+  rewrite Bool.andb_true_l.
+  destruct (con1 =? con2)%Z eqn:E.
+  + apply Z.eqb_eq in E.
+    contradiction.
+  + unfold negb.
+    rewrite H0.
+    reflexivity.
+Qed.
 
 Lemma proof_of_alpha_equiv_return_wit_3_2 : alpha_equiv_return_wit_3_2.
-Proof. Admitted. 
+Proof.
+  pre_process.
+  unfold store_term.
+  rewrite H4, H5.
+  entailer!.
+  unfold term_eqn, term_eqb.
+  rewrite H1 at 1.
+  rewrite Z.eqb_refl.
+  rewrite Bool.andb_true_l.
+  destruct (con1 =? con2)%Z eqn:E.
+  + unfold negb.
+    rewrite H0.
+    reflexivity. 
+  + apply Z.eqb_neq in E.
+    contradiction.
+Qed.
 
 Lemma proof_of_alpha_equiv_return_wit_4 : alpha_equiv_return_wit_4.
-Proof. Admitted. 
+Proof.
+  pre_process.
+  unfold store_term.
+  rewrite H3, H4.
+  entailer!.
+  unfold term_eqn, term_eqb.
+  rewrite H0 at 1.
+  rewrite Z.eqb_refl.
+  rewrite Bool.andb_true_l.
+  destruct (con1 =? con2)%Z eqn:E.
+  + unfold negb.
+    destruct (ctID typ1 =? 0)%Z eqn:Eq; [ | reflexivity].
+    apply Z.eqb_eq in E, Eq.
+    contradiction.
+  + unfold negb.
+    apply Z.eqb_neq in E.
+    destruct (ctID typ1 =? 0)%Z eqn:Eq; [ | reflexivity].
+    apply Z.eqb_eq in Eq.
+    contradiction.
+Qed.  
 
 Lemma proof_of_alpha_equiv_return_wit_5_1 : alpha_equiv_return_wit_5_1.
-Proof. Admitted. 
+Proof.
+  pre_process.
+  unfold store_term.
+  rewrite H5, H6.
+  fold store_term.
+  Exists y1 z1 y2 z2.
+  entailer!.
+  unfold term_eqn in *.
+  unfold term_eqb.
+  fold term_eqb.
+  destruct (term_eqb rt1 rt2) eqn:Eqr; [ | contradiction].
+  destruct (term_eqb lt1 lt2) eqn:Eql; [ | contradiction].
+  reflexivity.
+Qed.
 
 Lemma proof_of_alpha_equiv_return_wit_5_2 : alpha_equiv_return_wit_5_2.
-Proof. Admitted. 
+Proof.
+  pre_process.
+  unfold store_term.
+  rewrite H5, H6.
+  fold store_term.
+  Exists y1 z1 y2 z2.
+  entailer!.
+  unfold term_eqn in *.
+  unfold term_eqb.
+  fold term_eqb.
+  destruct (term_eqb lt1 lt2) eqn:Eql; [ | contradiction].
+  destruct (term_eqb rt1 rt2) eqn:Eqr; [ | reflexivity].
+  congruence.
+Qed.
 
 Lemma proof_of_alpha_equiv_return_wit_5_3 : alpha_equiv_return_wit_5_3.
-Proof. Admitted. 
+Proof.
+  pre_process.
+  unfold store_term.
+  rewrite H3, H4.
+  fold store_term.
+  Exists y1 z1 y2 z2.
+  entailer!.
+  unfold term_eqn in *.
+  unfold term_eqb.
+  fold term_eqb.
+  destruct (term_eqb lt1 lt2) eqn:Eql; [ | reflexivity].
+  congruence.
+Qed.
 
 Lemma proof_of_alpha_equiv_return_wit_6 : alpha_equiv_return_wit_6.
-Proof. Admitted. 
+Proof.
+  pre_process.
+  unfold store_term.
+  rewrite H2, H3.
+  fold store_term.
+  Exists y1 z1 y2 z2.
+  entailer!.
+  unfold term_eqn in *.
+  unfold term_eqb.
+  fold term_eqb.
+  destruct (qtID qt1 =? qtID qt2)%Z eqn:Eq; [ | reflexivity].
+  apply Z.eqb_eq in Eq.
+  congruence.
+Qed.
 
 Lemma proof_of_alpha_equiv_return_wit_7 : alpha_equiv_return_wit_7.
-Proof. Admitted. 
+Proof.
+  pre_process.
+  unfold store_term.
+  rewrite H5, H6.
+  fold store_term.
+  Exists y1 z1 y2 z2.
+  entailer!.
+  unfold term_eqn in *.
+  unfold term_eqb.
+  fold term_eqb.
+  rewrite H0 in H1. 
+  unfold list_Z_cmp in H1.
+  destruct (qtID qt1 =? qtID qt2)%Z eqn:Eq.
+  + destruct (list_Z_eqb qv1 qv2) eqn:vEq; [ | congruence].
+    rewrite Bool.andb_true_l.
+    tauto.
+  + destruct (list_Z_eqb qv1 qv2) eqn:vEq; [ | congruence].
+    rewrite Z.eqb_neq in Eq.
+    congruence.
+Qed.
 
 Lemma proof_of_alpha_equiv_return_wit_8 : alpha_equiv_return_wit_8.
-Proof. Admitted. 
+Proof.
+  pre_process.
+  unfold store_term.
+  rewrite H9, H10.
+  fold store_term.
+  Exists y1 z1 y2 z2.
+  entailer!.  
+  unfold term_eqn in *.
+  unfold term_eqb.
+  fold term_eqb.
+  Admitted. 
 
 Lemma proof_of_alpha_equiv_return_wit_9_1 : alpha_equiv_return_wit_9_1.
 Proof. Admitted. 
